Cleaned up clauses

src/cnf/clause.lean
@@ -1,7 +1,6 @@
 /-
 This file contains the definition of a Boolean (disjunctive) clause.
-This particular implementation has clauses as lists, although a set definition
-is sufficient as well.
+This particular implementation has clauses as lists.
 
 Authors: Cayden Codel, Jeremy Avigad, Marijn Heule
 Carnegie Mellon Univeristy
@@ -16,7 +15,7 @@ import data.list.basic
 universe u
 
 -- Represents the parametric type of the variable stored in the literal
-variables {V : Type*} [decidable_eq V] [inhabited V]
+variables {V : Type*}
 
 /- Disjunctive clauses are lists of literals, joined by logical ORs. -/
 def clause (V : Type*) := list (literal V)
@@ -35,9 +34,9 @@ open list
 
 -- Many of these properties follow directly from lists
 
-instance : inhabited (clause V) := ⟨[arbitrary (literal V)]⟩
+instance [inhabited V] : inhabited (clause V) := ⟨[arbitrary (literal V)]⟩
 
-instance has_decidable_eq : decidable_eq (clause V)
+instance has_decidable_eq [decidable_eq V] : decidable_eq (clause V)
 | []        []        := is_true rfl
 | (a :: as) []        := is_false (λ h, list.no_confusion h)
 | []        (b :: bs) := is_false (λ h, list.no_confusion h)
@@ -53,42 +52,33 @@ instance has_decidable_eq : decidable_eq (clause V)
 
 instance : has_mem (literal V) (clause V) := ⟨list.mem⟩
 instance : has_emptyc (clause V) := ⟨list.nil⟩ -- Refactor empty into [] below?
-instance : has_union (clause V) := ⟨list.union⟩
-instance : has_inter (clause V) := ⟨list.inter⟩
+instance [decidable_eq V] : has_union (clause V) := ⟨list.union⟩
+instance [decidable_eq V] : has_inter (clause V) := ⟨list.inter⟩
 instance : has_singleton (literal V) (clause V) := ⟨λ l, [l]⟩ 
-instance : has_insert (literal V) (clause V) := ⟨list.insert⟩
+instance [decidable_eq V] : has_insert (literal V) (clause V) := ⟨list.insert⟩
 instance : has_append (clause V) := ⟨list.append⟩
 instance : has_subset (clause V) := ⟨list.subset⟩
 instance [has_repr V] : has_repr (clause V) := ⟨list.repr⟩
 
-instance (l : literal V) (c : clause V) : decidable (l ∈ c) :=
+instance [decidable_eq V] (l : literal V) (c : clause V) : decidable (l ∈ c) :=
 by apply_instance
 
 /-! # eval -/
+section eval
 
--- Note: protected b/c many constructs will have an evaluation def
-/- To evaluate the clause, fold false along until a true evaluation is found -/
-protected def eval (τ : assignment V) (c : clause V) : bool :=
-  c.foldr (λ l b, b || (l.eval τ)) ff
+variables (τ : assignment V) (l : literal V) (c c₁ c₂ : clause V)
 
--- Proving properties of the fold operation
-lemma eval_op_left_comm (τ : assignment V) : 
-  left_commutative (λ (l : literal V) (b : bool), b || (l.eval τ)) :=
-assume l₁ l₂ b, by simp [bool.bor_comm, bool.bor_assoc]
+protected def eval : bool := c.foldr (λ l b, b || (l.eval τ)) ff
 
-@[simp] theorem eval_nil (τ : assignment V) : clause.eval τ [] = ff := rfl
+@[simp] theorem eval_nil : clause.eval τ [] = ff := rfl
 
-@[simp] theorem eval_singleton (τ : assignment V) (l : literal V) : 
-  clause.eval τ [l] = l.eval τ :=
+@[simp] theorem eval_singleton : clause.eval τ [l] = l.eval τ :=
 by simp only [clause.eval, foldr, ff_bor]
 
--- TODO make this, and other similarly-named theorems, protected?
-theorem eval_cons (τ : assignment V) (l : literal V) (c : clause V) : 
-  clause.eval τ (l :: c) = (literal.eval τ l) || (clause.eval τ c) :=
+@[simp] theorem eval_cons : clause.eval τ (l :: c) = (l.eval τ) || (c.eval τ) :=
 by simp only [clause.eval, foldr, bool.bor_comm]
 
-theorem eval_append (τ : assignment V) (c₁ c₂ : clause V) :
-  clause.eval τ (c₁ ++ c₂) = c₁.eval τ || c₂.eval τ :=
+theorem eval_append : clause.eval τ (c₁ ++ c₂) = c₁.eval τ || c₂.eval τ :=
 begin
   unfold clause.eval,
   rw foldr_append,
@@ -98,48 +88,29 @@ begin
 end
 
 theorem eval_tt_iff_exists_literal_eval_tt {τ : assignment V} {c : clause V} : 
-  c.eval τ = tt ↔ ∃ l ∈ c, literal.eval τ l = tt :=
+  c.eval τ = tt ↔ ∃ l, l ∈ c ∧ literal.eval τ l = tt :=
 begin
-  split,
-  { induction c with l ls ih,
-    { contradiction },
-    { simp [eval_cons],
-      intro h, cases h,
-      { use [l, h] },
-      { rcases ih h with ⟨l₂, hl, he⟩,
-        use [l₂, mem_cons_of_mem l hl, he] } } },
-  { rintros ⟨l, hl, he⟩,
-    induction c with d ds ih,
-    { exact absurd hl (not_mem_nil _) },
-    { rcases eq_or_ne_mem_of_mem hl with rfl | ⟨hne, hds⟩,
-      { simp [eval_cons, he] },
-      { simp [eval_cons, ih hds] } } }
-end
-
-theorem ne_nil_of_eval_tt {τ : assignment V} {c : clause V} :
-  c.eval τ = tt → c ≠ [] :=
-begin
-  intro h,
-  rcases eval_tt_iff_exists_literal_eval_tt.mp h with ⟨l, hmem, _⟩,
-  exact ne_nil_of_mem hmem
+  induction c with l ls ih,
+  { simp only [eval_nil, not_mem_nil, false_and, exists_false] },
+  { simp only [eval_cons, bor_eq_true_eq_eq_tt_or_eq_tt, mem_cons_iff],
+    split,
+    { rintros (h | h),
+      { use [l, or.inl rfl, h] },
+      { rcases ih.mp h with ⟨l₂, hl, he⟩,
+        use [l₂, mem_cons_of_mem l hl, he] } },
+    { rintros ⟨l₂, (rfl | hl), he⟩,
+      { exact or.inl he },
+      { exact or.inr (ih.mpr ⟨l₂, hl, he⟩) } } }
 end
 
 theorem eval_ff_iff_forall_literal_eval_ff {τ : assignment V} {c : clause V} : 
-  clause.eval τ c = ff ↔ ∀ l ∈ c, literal.eval τ l = ff :=
+  clause.eval τ c = ff ↔ ∀ l, l ∈ c → literal.eval τ l = ff :=
 begin
-  split,
-  { induction c with l ls ih,
-    { intros _ l hl, exact absurd hl (not_mem_nil l) },
-    { simp [eval_cons],
-      intros hl hds,
-      exact and.intro hl (ih hds) } },
-  { induction c with l ls ih,
-    { rw eval_nil, tautology },
-    { intro h,
-      simp [eval_cons, h l (mem_cons_self l ls)],
-      have : ∀ (m : literal V), m ∈ ls → literal.eval τ m = ff,
-      { intros m hm, exact h m (mem_cons_of_mem l hm) },
-      exact ih this } }
+  induction c with l ls ih,
+  { simp only [eval_nil, eq_self_iff_true, not_mem_nil, is_empty.forall_iff, implies_true_iff] },
+  { simp only [eval_cons, bor_eq_false_eq_eq_ff_and_eq_ff, mem_cons_iff, 
+      forall_eq_or_imp, and.congr_right_iff],
+    intro _, exact ih }
 end
 
 theorem eval_tautology {c : clause V} {l : literal V} : 
@@ -148,11 +119,9 @@ begin
   intros hl hlf τ,
   apply eval_tt_iff_exists_literal_eval_tt.mpr,
   cases h : (literal.eval τ l),
-  { use [l.flip, hlf, eval_flip_of_eval h] },
-  { use [l, hl, h] }
+  { exact ⟨l.flip, hlf, eval_flip_of_eval h⟩ },
+  { exact ⟨l, hl, h⟩ }
 end
-
--- Evaluation of subsets and sublists tie in to evaluation nicely
 
 theorem eval_tt_of_subset_eval_tt {τ : assignment V} {c₁ c₂ : clause V} :
   c₁ ⊆ c₂ → clause.eval τ c₁ = tt → clause.eval τ c₂ = tt :=
@@ -160,7 +129,7 @@ begin
   intros h₁ h₂,
   apply eval_tt_iff_exists_literal_eval_tt.mpr,
   rcases eval_tt_iff_exists_literal_eval_tt.mp h₂ with ⟨l, hl, he⟩,
-  use [l, h₁ hl, he]
+  exact ⟨l, h₁ hl, he⟩
 end
 
 theorem eval_ff_of_superset_eval_ff {τ : assignment V} {c₁ c₂ : clause V} :
@@ -169,8 +138,7 @@ begin
   intros h₁ h₂,
   apply eval_ff_iff_forall_literal_eval_ff.mpr,
   intros l hl,
-  rw eval_ff_iff_forall_literal_eval_ff at h₂,
-  exact h₂ l (h₁ hl)
+  exact (eval_ff_iff_forall_literal_eval_ff.mp h₂) l (h₁ hl)
 end
 
 theorem eval_tt_of_sublist_eval_tt {τ : assignment V} {c₁ c₂ : clause V} :
@@ -181,100 +149,96 @@ theorem eval_ff_of_superlist_eval_ff {τ : assignment V} {c₁ c₂ : clause V} 
   c₁ <+ c₂ → clause.eval τ c₂ = ff → clause.eval τ c₁ = ff :=
 assume h₁, eval_ff_of_superset_eval_ff (sublist.subset h₁)
 
-theorem eval_tt_cons_of_eval_tt 
-  {τ : assignment V} {c : clause V} (l : literal V) :
+theorem eval_tt_cons_of_eval_tt {τ : assignment V} {c : clause V} (l : literal V) :
   clause.eval τ c = tt → clause.eval τ (l :: c) = tt :=
 assume h, eval_tt_of_sublist_eval_tt (sublist_cons l c) h
 
-theorem eval_ff_of_eval_ff_cons 
-  {τ : assignment V} {c : clause V} {l : literal V} :
+theorem eval_ff_of_eval_ff_cons {τ : assignment V} {c : clause V} {l : literal V} :
   clause.eval τ (l :: c) = ff → clause.eval τ c = ff :=
 assume h, eval_ff_of_superlist_eval_ff (sublist_cons l c) h
 
+end eval
+
 /-! ### Counting -/
+section counting
 
-/- Counts the number of literals that evaluate to true, under τ -/
-protected def count_tt (τ : assignment V) (c : clause V) : nat :=
-  c.countp (literal.is_true τ)
+variables (τ : assignment V) (l : literal V) (c c₁ c₂ : clause V)
 
-/- Counts the number of literals that evaluate to false, under τ -/
-protected def count_ff (τ : assignment V) (c : clause V) : nat :=
-  c.countp (literal.is_false τ)
+protected def count_tt : nat := c.countp (literal.is_true τ)
+protected def count_ff : nat := c.countp (literal.is_false τ)
 
-/- Counts the number of positive literals in the clause -/
-def count_pos (c : clause V) : nat :=
-  c.countp literal.is_pos
+def count_pos (c : clause V) : nat := c.countp literal.is_pos
+def count_neg (c : clause V) : nat := c.countp literal.is_neg
 
-/- Counts the number of negative literals in the clause -/
-def count_neg (c : clause V) : nat :=
-  c.countp literal.is_neg
-
-@[simp] lemma count_tt_nil (τ : assignment V) : clause.count_tt τ [] = 0 := rfl
-@[simp] lemma count_ff_nil (τ : assignment V) : clause.count_ff τ [] = 0 := rfl
+@[simp] lemma count_tt_nil : clause.count_tt τ [] = 0 := rfl
+@[simp] lemma count_ff_nil : clause.count_ff τ [] = 0 := rfl
 @[simp] lemma count_pos_nil : count_pos ([] : clause V) = 0 := rfl
 @[simp] lemma count_neg_nil : count_neg ([] : clause V) = 0 := rfl
 
-@[simp] theorem count_tt_singleton (τ : assignment V) (l : literal V) :
-  clause.count_tt τ [l] = cond (l.eval τ) 1 0 :=
-by cases h : (l.eval τ); { simp [h, clause.count_tt, literal.is_true] }
+@[simp] theorem count_tt_singleton : clause.count_tt τ [l] = cond (l.eval τ) 1 0 :=
+by cases h : (l.eval τ); simp [h, clause.count_tt, literal.is_true]
 
-@[simp] theorem count_ff_singleton (τ : assignment V) (l : literal V) :
-  clause.count_ff τ [l] = cond (l.eval τ) 0 1 :=
-by cases h : (l.eval τ); { simp [h, clause.count_ff, literal.is_false] }
+@[simp] theorem count_ff_singleton : clause.count_ff τ [l] = cond (l.eval τ) 0 1 :=
+by cases h : (l.eval τ); simp [h, clause.count_ff, literal.is_false]
 
-@[simp] theorem count_pos_singleton (l : literal V) :
-  count_pos [l] = cond l.is_pos 1 0 :=
+@[simp] theorem count_pos_singleton : count_pos [l] = cond l.is_pos 1 0 :=
 by cases l; simp [count_pos, literal.is_pos]
 
-@[simp] theorem count_neg_singleton (l : literal V) :
-  count_neg [l] = cond l.is_neg 1 0 :=
+@[simp] theorem count_neg_singleton : count_neg [l] = cond l.is_neg 1 0 :=
 by cases l; simp [count_neg, literal.is_neg]
 
-theorem count_tt_cons (τ : assignment V) (l : literal V) (c : clause V) :
-  clause.count_tt τ (l :: c) = cond (l.eval τ) (1 + c.count_tt τ) (c.count_tt τ) :=
-by cases h : (literal.eval τ l); 
-  { simp [h, literal.is_true, clause.count_tt, add_comm] }
+@[simp] theorem count_tt_cons : clause.count_tt τ (l :: c) = cond (l.eval τ) (1 + c.count_tt τ) (c.count_tt τ) :=
+by cases h : (l.eval τ); simp [h, literal.is_true, clause.count_tt, add_comm]
 
-theorem count_ff_cons (τ : assignment V) (l : literal V) (c : clause V) :
-  clause.count_ff τ (l :: c) = cond (l.eval τ) (c.count_ff τ) (1 + c.count_ff τ) :=
-by cases h : (literal.eval τ l);
-  { simp [h, literal.is_false, clause.count_ff, add_comm] }
+@[simp] theorem count_ff_cons : clause.count_ff τ (l :: c) = cond (l.eval τ) (c.count_ff τ) (1 + c.count_ff τ) :=
+by cases h : (l.eval τ); simp [h, literal.is_false, clause.count_ff, add_comm]
 
-theorem count_pos_cons (l : literal V) (c : clause V) :
-  count_pos (l :: c) = cond l.is_pos (1 + c.count_pos) c.count_pos :=
-by cases l; { simp [count_pos, literal.is_pos, add_comm] }
+@[simp] theorem count_pos_cons : count_pos (l :: c) = cond l.is_pos (1 + c.count_pos) c.count_pos :=
+by cases l; simp [count_pos, literal.is_pos, add_comm]
 
-theorem count_neg_cons (l : literal V) (c : clause V) :
-  count_neg (l :: c) = cond l.is_neg (1 + c.count_neg) c.count_neg :=
-by cases l; { simp [count_neg, literal.is_neg, add_comm] }
+@[simp] theorem count_neg_cons : count_neg (l :: c) = cond l.is_neg (1 + c.count_neg) c.count_neg :=
+by cases l; simp [count_neg, literal.is_neg, add_comm]
 
-theorem count_tt_append (τ : assignment V) (c₁ c₂ : clause V) :
-  clause.count_tt τ (c₁ ++ c₂) = clause.count_tt τ c₁ + clause.count_tt τ c₂ :=
+theorem count_tt_append : clause.count_tt τ (c₁ ++ c₂) = clause.count_tt τ c₁ + clause.count_tt τ c₂ :=
 begin
   induction c₁ with l ls ih,
   { simp only [count_tt_nil, zero_add, nil_append] },
-  { cases h : (literal.eval τ l);
-    { simp [count_tt_cons, h, ih, add_assoc] } }
+  { cases h : (literal.eval τ l); simp [h, ih, add_assoc] }
 end
 
--- Can make analogous append theorems for each of the others
+theorem count_ff_append : clause.count_ff τ (c₁ ++ c₂) = clause.count_ff τ c₁ + clause.count_ff τ c₂ :=
+begin
+  induction c₁ with l ls ih,
+  { simp only [count_ff_nil, zero_add, nil_append] },
+  { cases h : (literal.eval τ l); { simp [h, ih, add_assoc] } }
+end
 
--- All the above four functions are capped by the length of the clause
-theorem count_tt_le_length (τ : assignment V) (c : clause V) :
-  c.count_tt τ ≤ c.length :=
+theorem count_pos_append : clause.count_pos (c₁ ++ c₂) = clause.count_pos c₁ + clause.count_pos c₂ :=
+begin
+  induction c₁ with l ls ih,
+  { simp only [nil_append, count_pos_nil, zero_add] },
+  { cases l; simp [ih, literal.is_pos, add_assoc] }
+end
+
+theorem count_neg_append : clause.count_neg (c₁ ++ c₂) = clause.count_neg c₁ + clause.count_neg c₂ :=
+begin
+  induction c₁ with l ls ih,
+  { simp only [nil_append, count_neg_nil, zero_add] },
+  { cases l; { simp [ih, literal.is_neg, add_assoc] } }
+end
+
+theorem count_tt_le_length : c.count_tt τ ≤ c.length :=
 by simp only [clause.count_tt, countp_eq_length_filter, length_filter]
 
-theorem count_ff_le_length (τ : assignment V) (c : clause V) : 
-  c.count_ff τ ≤ c.length :=
+theorem count_ff_le_length : c.count_ff τ ≤ c.length :=
 by simp only [clause.count_ff, countp_eq_length_filter, length_filter]
 
-theorem count_pos_le_length (c : clause V) : c.count_pos ≤ c.length :=
+theorem count_pos_le_length : c.count_pos ≤ c.length :=
 by simp only [count_pos, countp_eq_length_filter, length_filter]
 
-theorem count_neg_le_length (c : clause V) : c.count_neg ≤ c.length :=
+theorem count_neg_le_length : c.count_neg ≤ c.length :=
 by simp only [count_neg, countp_eq_length_filter, length_filter]
 
--- count_tt and count_ff are complements of each other
 theorem count_tt_plus_count_ff_eq_length (τ : assignment V) (c : clause V) :
   c.count_tt τ + c.count_ff τ = c.length :=
 begin
@@ -282,277 +246,202 @@ begin
   { simp },
   { cases h : (l.eval τ);
     simp [count_tt_cons, count_ff_cons, h, ← ih],
-    { rw add_assoc,
-      rw add_comm (clause.count_ff τ ls) 1 },
-    { rw add_comm (clause.count_tt τ ls + clause.count_ff τ ls) 1,
-      rw ← add_assoc } }
+    { rw [add_assoc, add_comm (clause.count_ff τ ls) 1] },
+    { rw [add_comm (clause.count_tt τ ls + clause.count_ff τ ls) 1, ← add_assoc] } }
 end
 
-theorem count_tt_eq_length_sub_count_ff (τ : assignment V) (c : clause V) :
-  c.count_tt τ = c.length - c.count_ff τ :=
+theorem count_tt_eq_length_sub_count_ff : c.count_tt τ = c.length - c.count_ff τ :=
 eq_tsub_of_add_eq (count_tt_plus_count_ff_eq_length τ c)
 
-theorem count_ff_eq_length_sub_count_tt (τ : assignment V) (c : clause V) :
-  c.count_ff τ = c.length - c.count_tt τ :=
-begin
-  have := count_tt_plus_count_ff_eq_length τ c,
-  rw add_comm at this,
-  exact eq_tsub_of_add_eq this
-end
+theorem count_ff_eq_length_sub_count_tt : c.count_ff τ = c.length - c.count_tt τ :=
+eq_tsub_of_add_eq (add_comm (c.count_tt τ) (c.count_ff τ) ▸ count_tt_plus_count_ff_eq_length τ c)
 
--- count_pos and count_neg are complements of each other
-theorem count_pos_plus_count_neg_eq_length (c : clause V) :
-  c.count_pos + c.count_neg = c.length :=
+theorem count_pos_plus_count_neg_eq_length : c.count_pos + c.count_neg = c.length :=
 begin
   induction c with l ls ih,
   { simp },
   { cases l;
     simp [count_pos_cons, count_neg_cons, literal.is_pos, literal.is_neg, ← ih],
-    { rw add_comm (count_pos ls + count_neg ls) 1,
-      rw ← add_assoc },
-    { rw add_assoc,
-      rw add_comm 1 } }
+    { rw [add_comm (count_pos ls + count_neg ls) 1, ← add_assoc] },
+    { rw [add_assoc, add_comm 1] } }
 end
 
-theorem count_pos_eq_length_sub_count_neg (c : clause V) :
-  c.count_pos = c.length - c.count_neg :=
+theorem count_pos_eq_length_sub_count_neg : c.count_pos = c.length - c.count_neg :=
 eq_tsub_of_add_eq (count_pos_plus_count_neg_eq_length c)
 
-theorem count_neg_eq_length_sub_count_pos (c : clause V) :
-  c.count_neg = c.length - c.count_pos :=
+theorem count_neg_eq_length_sub_count_pos : c.count_neg = c.length - c.count_pos :=
+eq_tsub_of_add_eq (add_comm (c.count_pos) (c.count_neg) ▸ count_pos_plus_count_neg_eq_length c)
+
+theorem count_tt_eq_zero_iff_eval_ff {τ : assignment V} {c : clause V} : 
+  c.count_tt τ = 0 ↔ c.eval τ = ff :=
 begin
-  have := count_pos_plus_count_neg_eq_length c,
-  rw add_comm at this,
-  exact eq_tsub_of_add_eq this
+  rw [clause.count_tt, countp_eq_zero, eval_ff_iff_forall_literal_eval_ff],
+  split,
+  { intros hc l hl,
+    have := hc l hl,
+    rw [literal.is_true, eq_ff_eq_not_eq_tt] at this,
+    exact this },
+  { intros hl a ha, simp [literal.is_true, hl a ha] }
 end
 
--- Note: A good countp lemma may reduce the forward direction
-theorem count_tt_eq_zero_iff_eval_ff {τ : assignment V} {c : clause V} :
-  c.eval τ = ff ↔ c.count_tt τ = 0 :=
+theorem count_tt_gt_zero_iff_eval_tt {τ : assignment V} {c : clause V} :
+  c.count_tt τ > 0 ↔ c.eval τ = tt :=
 begin
+  rw [clause.count_tt, eval_tt_iff_exists_literal_eval_tt],
   split,
-  { induction c with l ls ih,
-    { simp },
-    { simp [eval_cons, count_tt_cons],
-      intros hl hls,
-      simp [hl, ih hls] } },
-  { induction c with l ls ih,
-    { simp },
-    { simp [eval_cons, count_tt_cons],
-      have : 1 + clause.count_tt τ ls ≠ 0,
-      { rw add_comm,
-        rw ← nat.succ_eq_add_one,
-        exact nat.succ_ne_zero _ },
-      intro h,
-      have := ff_of_ne_first_of_cond_eq this h,
-      simp [this] at h,
-      exact and.intro this (ih h) } }
+  { intro hp,
+    rcases (countp_pos _).mp hp with ⟨l, hl, he⟩,
+    exact ⟨l, hl, he⟩ },
+  { rintro ⟨l, hl, he⟩,
+    exact (countp_pos _).mpr ⟨l, hl, he⟩ } 
 end
 
-theorem count_tt_eval_tt_iff_gt_zero {τ : assignment V} {c : clause V} :
-  c.eval τ = tt ↔ clause.count_tt τ c > 0 :=
-begin
-  split,
-  { intro h,
-    apply (countp_pos _).mpr,
-    use eval_tt_iff_exists_literal_eval_tt.mp h },
-  { intro h,
-    apply eval_tt_iff_exists_literal_eval_tt.mpr,
-    use (countp_pos _).mp h } 
-end
+end counting
 
 /-! # falsify and truthify -/
+section falsify
 
--- For any assignment and variables, there is a false clause on those variables
+variables (τ : assignment V) (v : V) (l : list V) {c c₁ c₂ : clause V}
+
+-- For any assignment and variables, there is a clause that evaluates to false
 -- Simply map each variable in the list to the literal which evaluates to false
-def falsify (τ : assignment V) (l : list V) : clause V :=
-l.map (λ v, cond (τ v) (Neg v) (Pos v))
+def falsify : clause V := l.map (λ v, cond (τ v) (Neg v) (Pos v))
+def truthify : clause V := l.map (λ v, cond (τ v) (Pos v) (Neg v))
 
--- For any assignment and variables, there is a true clause on those variables
--- Note: there is no such clause for the empty set of variables
-def truthify (τ : assignment V) (l : list V) : clause V :=
-l.map (λ v, cond (τ v) (Pos v) (Neg v))
+@[simp] lemma falsify_nil : falsify τ [] = [] := rfl
+@[simp] lemma truthify_nil : truthify τ [] = [] := rfl
 
-@[simp] lemma falsify_nil (τ : assignment V) : falsify τ [] = [] := rfl
-@[simp] lemma truthify_nil (τ : assignment V) : truthify τ [] = [] := rfl
+@[simp] lemma falsify_singleton : falsify τ [v] = cond (τ v) [Neg v] [Pos v] :=
+by cases h : τ v; simp [h, falsify]
 
-@[simp] lemma falsify_singleton (τ : assignment V) (v : V) :
-  falsify τ [v] = cond (τ v) [Neg v] [Pos v] :=
-by cases h : τ v; { simp [h, falsify] }
+@[simp] lemma truthify_singleton : truthify τ [v] = cond (τ v) [Pos v] [Neg v] :=
+by cases h : τ v; simp [h, truthify]
 
-@[simp] lemma truthify_singleton (τ : assignment V) (v : V) :
-  truthify τ [v] = cond (τ v) [Pos v] [Neg v] :=
-by cases h : τ v; { simp [h, truthify] }
+@[simp] theorem falsify_cons : falsify τ (v :: l) = cond (τ v) (Neg v :: falsify τ l) (Pos v :: falsify τ l) :=
+by cases h : τ v; simp [falsify, map_cons, h]
 
-theorem falsify_cons (τ : assignment V) (v : V) (vs : list V) :
-  falsify τ (v :: vs) = cond (τ v) (Neg v :: falsify τ vs)
-                                   (Pos v :: falsify τ vs) :=
-by cases h : τ v; { simp [falsify, map_cons, h] }
+@[simp] theorem truthify_cons : truthify τ (v :: l) = cond (τ v) (Pos v :: truthify τ l) (Neg v :: truthify τ l) :=
+by cases h : τ v; simp [truthify, map_cons, h]
 
-theorem truthify_cons (τ : assignment V) (v : V) (vs : list V) :
-  truthify τ (v :: vs) = cond (τ v) (Pos v :: truthify τ vs)
-                                    (Neg v :: truthify τ vs) :=
-by cases h : τ v; { simp [truthify, map_cons, h] }
-
-theorem falsify_eval_ff (τ : assignment V) (l : list V) :
-  clause.eval τ (falsify τ l) = ff :=
+theorem falsify_eval_ff : clause.eval τ (falsify τ l) = ff :=
 begin
   induction l with v vs ih,
-  { rw falsify_nil, rw eval_nil },
-  { cases h : (τ v);
-    { simp [falsify_cons, h, eval_cons, literal.eval, ih] } }
+  { rw [falsify_nil, eval_nil] },
+  { cases h : (τ v); simp [h, eval_cons, literal.eval, ih] }
 end
 
-theorem truthify_eval_tt (τ : assignment V) {l : list V} (hl : l ≠ []) : 
-  clause.eval τ (truthify τ l) = tt :=
+theorem truthify_eval_tt {l : list V} (hl : l ≠ []) : clause.eval τ (truthify τ l) = tt :=
 begin
   induction l with v vs ih,
   { contradiction },
-  { cases h : (τ v);
-    { simp [truthify_cons, h, literal.eval, eval_cons] } }
+  { cases h : (τ v); simp [h, literal.eval, eval_cons] }
 end
 
-theorem flip_truthify_eq_falsify (τ : assignment V) (l : list V) : 
-  map literal.flip (truthify τ l) = falsify τ l :=
+theorem flip_truthify_eq_falsify : map literal.flip (truthify τ l) = falsify τ l :=
 begin
   induction l with v vs ih,
-  { simp },
-  { cases h : (τ v);
-    { simp [h, literal.eval, ih, literal.flip, truthify_cons, falsify_cons] } }
+  { refl },
+  { cases h : (τ v); simp [h, literal.eval, ih, literal.flip] }
 end
 
--- If falsify/truthify become type (fin)set, these theorems aren't needed
-theorem falsify_map_var_eq (τ : assignment V) (l : list V) : 
-  map var (falsify τ l) = l :=
+theorem falsify_map_var_eq : map var (falsify τ l) = l :=
 begin
   induction l with v vs ih,
-  { simp only [falsify_nil, map_nil] },
+  { refl },
   { cases h : (τ v);
-    { simp only [falsify_cons, map_cons, h, var, 
-        true_and, eq_self_iff_true, cond],
+    { simp only [falsify_cons, map_cons, h, var, true_and, eq_self_iff_true, cond],
       exact ih } }
 end
 
-theorem truthify_map_var_eq (τ : assignment V) (l : list V) :
-  map var (truthify τ l) = l :=
+theorem truthify_map_var_eq : map var (truthify τ l) = l :=
 begin
   induction l with v vs ih,
-  { simp only [truthify_nil, map_nil] },
+  { refl },
   { cases h : (τ v);
-    { simp only [truthify_cons, map_cons, h, var, 
-        true_and, eq_self_iff_true, cond],
+    { simp only [truthify_cons, map_cons, h, var, true_and, eq_self_iff_true, cond],
       exact ih } }
 end
 
-theorem count_tt_falsify (τ : assignment V) (l : list V) :
-  clause.count_tt τ (falsify τ l) = 0 :=
-count_tt_eq_zero_iff_eval_ff.mp (falsify_eval_ff τ l)
+theorem count_tt_falsify : clause.count_tt τ (falsify τ l) = 0 :=
+count_tt_eq_zero_iff_eval_ff.mpr (falsify_eval_ff τ l)
 
-lemma count_tt_truthify (τ : assignment V) (l : list V) :
-  clause.count_tt τ (truthify τ l) = length l :=
+lemma count_tt_truthify : clause.count_tt τ (truthify τ l) = length l :=
 begin
   induction l with v vs ih,
-  { simp },
-  { cases h : τ v;
-    { simp [truthify_cons, count_tt_cons, literal.eval, h, ih, add_comm] } }
+  { refl },
+  { cases h : τ v; simp [literal.eval, h, ih, add_comm] }
 end
 
--- Falsify negates those literals that, if positive, are true
-theorem count_tt_pos_eq_count_neg_falsify (τ : assignment V) (l : list V) :
-  clause.count_tt τ (map Pos l) = count_neg (falsify τ l) :=
-begin
-  induction l with v vs ih,
-  { simp },
-  { cases h : (τ v);
-    { simp [map_cons, count_tt_cons, falsify_cons, count_neg_cons, 
-        literal.eval, h, ih, literal.is_neg] } }
-end
-
--- Sublist theorems (can have subset theorems too)
-theorem count_pos_sublist {c₁ c₂ : clause V} : 
-  c₁ <+ c₂ → c₁.count_pos ≤ c₂.count_pos :=
-assume h, by simp [count_pos, sublist.countp_le literal.is_pos h]
-
-theorem count_neg_sublist {c₁ c₂ : clause V} :
-  c₁ <+ c₂ → c₁.count_neg ≤ c₂.count_neg :=
-assume h, by simp [count_neg, sublist.countp_le literal.is_neg h]
-
-theorem count_tt_sublist (τ : assignment V) {c₁ c₂ : clause V} :
-  c₁ <+ c₂ → c₁.count_tt τ ≤ c₂.count_tt τ :=
+theorem count_tt_sublist : c₁ <+ c₂ → c₁.count_tt τ ≤ c₂.count_tt τ :=
 assume h, by simp [clause.count_tt, sublist.countp_le (literal.is_true τ) h]
 
-theorem count_ff_sublist (τ : assignment V) {c₁ c₂ : clause V} :
-  c₁ <+ c₂ → c₁.count_ff τ ≤ c₂.count_ff τ :=
+theorem count_ff_sublist : c₁ <+ c₂ → c₁.count_ff τ ≤ c₂.count_ff τ :=
 assume h, by simp [clause.count_ff, sublist.countp_le (literal.is_false τ) h]
 
-theorem pos_count_pos_iff_exists_pos {c : clause V} :
-  c.count_pos > 0 ↔ ∃ l ∈ c, literal.is_pos l :=
-by simp [count_pos, countp_pos]
+theorem count_pos_sublist : c₁ <+ c₂ → c₁.count_pos ≤ c₂.count_pos :=
+assume h, by simp [count_pos, sublist.countp_le literal.is_pos h]
 
-theorem pos_count_neg_iff_exists_neg {c : clause V} :
-  c.count_neg > 0 ↔ ∃ l ∈ c, literal.is_neg l :=
-by simp [count_neg, countp_pos]
+theorem count_neg_sublist : c₁ <+ c₂ → c₁.count_neg ≤ c₂.count_neg :=
+assume h, by simp [count_neg, sublist.countp_le literal.is_neg h]
 
-theorem pos_count_tt_iff_exists_tt {τ : assignment V} {c : clause V} :
-  c.count_tt τ > 0 ↔ ∃ l ∈ c, literal.is_true τ l :=
+theorem pos_count_tt_iff_exists_tt {τ} : c.count_tt τ > 0 ↔ ∃ l, l ∈ c ∧ literal.is_true τ l :=
 by simp [clause.count_tt, countp_pos]
 
-theorem pos_count_ff_iff_exists_ff {τ : assignment V} {c : clause V} :
-  c.count_ff τ > 0 ↔ ∃ l ∈ c, literal.is_false τ l :=
+theorem pos_count_ff_iff_exists_ff {τ} : c.count_ff τ > 0 ↔ ∃ l, l ∈ c ∧ literal.is_false τ l :=
 by simp [clause.count_ff, countp_pos]
 
-theorem count_tt_perm {τ : assignment V} {c₁ c₂ : clause V} :
-  c₁ ~ c₂ → c₁.count_tt τ = c₂.count_tt τ :=
+theorem pos_count_pos_iff_exists_pos : c.count_pos > 0 ↔ ∃ l, l ∈ c ∧ literal.is_pos l :=
+by simp [count_pos, countp_pos]
+
+theorem pos_count_neg_iff_exists_neg : c.count_neg > 0 ↔ ∃ l, l ∈ c ∧ literal.is_neg l :=
+by simp [count_neg, countp_pos]
+
+theorem count_tt_perm : c₁ ~ c₂ → c₁.count_tt τ = c₂.count_tt τ :=
 begin
   intro hp,
   induction hp with x l₂ l₂' p IH  x y l₂  l₂ m₂ r₂ p₁ p₂ IH₁ IH₂,
   { refl },
   { simp [count_tt_cons, IH] },
-  { simp [count_tt_cons],
-    cases literal.eval τ x; { cases literal.eval τ y; simp } },
+  { simp [count_tt_cons], cases literal.eval τ x; cases literal.eval τ y; simp },
   { exact eq.trans IH₁ IH₂ }
 end
 
+end falsify
+
 /-! # Flip counting -/
+section flips
+
+variables [decidable_eq V]
 
 -- If two clauses have the same length, literals can be compared at each
 -- position. If they are literal.flip's of each other, increment a counter
-
--- Note: not good from a set perspective, as order must be maintained
-
 def count_flips : clause V → clause V → nat
 | []         _        := 0
 | _         []        := 0
 | (l :: ls) (m :: ms) := ite (l.flip = m) 
                          (1 + count_flips ls ms) (count_flips ls ms)
 
-@[simp] lemma count_flips_nil (c₁ c₂ : clause V) : 
-  c₁ = [] ∨ c₂ = [] → count_flips c₁ c₂ = 0 :=
-begin
-  intro h, rcases h with rfl | rfl, 
-  { cases c₂; { simp [count_flips] } },
-  { cases c₁; { simp [count_flips] } }
-end
+@[simp] lemma count_flips_nil (c : clause V) : count_flips [] c = 0 :=
+by cases c; refl
 
-theorem count_flips_cons (c₁ c₂ : clause V) (l₁ l₂ : literal V) :
+@[simp] theorem count_flips_cons (c₁ c₂ : clause V) (l₁ l₂ : literal V) :
   count_flips (l₁ :: c₁) (l₂ :: c₂) = ite (l₁.flip = l₂) 
     (1 + count_flips c₁ c₂) (count_flips c₁ c₂) :=
-by { by_cases l₁.flip = l₂; simp [count_flips, h] }
+by by_cases l₁.flip = l₂; simp only [count_flips]
 
-theorem count_flips_self (c : clause V) : count_flips c c = 0 :=
+@[simp] theorem count_flips_self (c : clause V) : count_flips c c = 0 :=
 begin
   induction c with l ls ih,
   { refl },
   { simp [count_flips, flip_ne, ih] }
 end
 
-lemma count_flips_comm (c₁ c₂ : clause V) : 
-  count_flips c₁ c₂ = count_flips c₂ c₁ :=
+theorem count_flips_comm (c₁ c₂ : clause V) : count_flips c₁ c₂ = count_flips c₂ c₁ :=
 begin
   induction c₁ with l ls ih generalizing c₂,
-  { simp },
+  { cases c₂; simp [count_flips] },
   { cases c₂,
-    { unfold count_flips },
+    { refl },
     { simp [count_flips, ih c₂_tl],
       by_cases h : (l.flip = c₂_hd),
       { simp [h, flip_eq_iff_eq_flip.mp h, flip_flip] },
@@ -562,11 +451,10 @@ end
 theorem count_flips_pos_of_map_var_eq_of_neq {c₁ c₂ : clause V} :
   map var c₁ = map var c₂ → c₁ ≠ c₂ → count_flips c₁ c₂ > 0 :=
 begin
+  intros h hne,
   induction c₁ with l ls ih generalizing c₂,
-  { intros h₁ h₂,
-    exact absurd (eq_nil_of_map_eq_nil h₁.symm).symm h₂ },
-  { intros h hne,
-    rcases exists_map_cons_of_map_cons h.symm with ⟨x, xs, rfl, hxl, hxs⟩,
+  { exact absurd (eq_nil_of_map_eq_nil h.symm).symm hne },
+  { rcases exists_map_cons_of_map_cons h.symm with ⟨x, xs, rfl, hxl, hxs⟩,
     unfold count_flips,
     rcases var_eq_iff_eq_or_flip_eq.mp hxl with rfl | rfl,
     { simp [ih (tail_eq_of_cons_eq h) (ne_tail_of_eq_head_of_ne hne rfl)] },
@@ -578,76 +466,37 @@ theorem count_flips_falsify_eq_count_tt (τ : assignment V) (c : clause V) :
 begin
   induction c with l ls ih,
   { simp },
-  { cases l;
-    { cases h : (τ l);
-      { simp [map_cons, falsify_cons, count_tt_cons, count_flips_cons, 
-          literal.eval, h, var, literal.flip, ih] } } }
+  { cases l; { cases h : (τ l); { simp [var, h, literal.eval, literal.flip, ih] } } }
 end
 
 /-! ## Parity reasoning for evaluation -/
 
-theorem eval_tt_of_tt_ne_neg_of_map_var_eq 
-  {τ : assignment V} {l : list V} {c : clause V} :
+theorem eval_tt_of_map_var_eq_of_tt_ne_neg {τ : assignment V} {l : list V} {c : clause V} :
   map var c = l → clause.count_tt τ (map Pos l) ≠ count_neg c → c.eval τ = tt :=
 begin
   induction l with v vs ih generalizing c,
   { rw map_eq_nil, rintro rfl, contradiction },
   { intros hc hne,
-    rcases exists_cons_of_map_cons hc with ⟨l, ls, rfl, hl, hls⟩,
+    rcases exists_cons_of_map_cons hc with ⟨l, ls, rfl, rfl, hls⟩,
     cases l,
-    { cases h : τ v,
-      { simp [map_cons, count_tt_cons, count_neg_cons, 
-          literal.is_neg, literal.eval, h] at hne,
+    { cases h : τ l,
+      { simp [literal.eval, var, literal.is_neg, h] at hne,
         exact eval_tt_cons_of_eval_tt _ (ih hls hne) },
-      { unfold var at hl,
-        simp [eval_cons, literal.eval, h, hl] } },
-    { cases h : τ v,
-      { unfold var at hl,
-        simp [eval_cons, literal.eval, h, hl] },
-      { simp [map_cons, count_tt_cons, count_neg_cons, 
-          literal.is_neg, literal.eval, h] at hne,
-        exact eval_tt_cons_of_eval_tt _ (ih hls hne) } } }
-end
-
--- Basically the same proof here as the one above
--- Take complement of count_ff, etc. to get above premises?
-theorem eval_tt_of_ff_ne_pos_of_map_var_eq 
-  {τ : assignment V} {l : list V} {c : clause V} : map var c = l 
-    → clause.count_ff τ (map Pos l) ≠ count_pos c → c.eval τ = tt :=
-begin
-  induction l with v vs ih generalizing c,
-  { rw map_eq_nil, rintro rfl, contradiction },
-  { intros hc hne,
-    rcases exists_cons_of_map_cons hc with ⟨l, ls, rfl, hl, hls⟩,
-    cases l,
-    { cases h : τ v,
-      { simp [map_cons, count_ff_cons, count_pos_cons, 
-          literal.is_pos, literal.eval, h] at hne,
-        exact eval_tt_cons_of_eval_tt _ (ih hls hne) },
-      { unfold var at hl,
-        simp [eval_cons, literal.eval, h, hl] } },
-    { cases h : τ v,
-      { unfold var at hl,
-        simp [eval_cons, literal.eval, h, hl] },
-      { simp [map_cons, count_ff_cons, count_pos_cons, 
-          literal.is_pos, literal.eval, h] at hne,
+      { simp [literal.eval, h] } },
+    { cases h : τ l,
+      { simp [literal.eval, h] },
+      { simp [literal.eval, var, literal.is_neg, h] at hne,
         exact eval_tt_cons_of_eval_tt _ (ih hls hne) } } }
 end
 
 -- Corollary of the above wrt parity reasoning
-theorem eval_tt_of_opposite_parity 
-  {τ : assignment V} {l : list V} {c : clause V} : map var c = l 
-    → nat.bodd (clause.count_tt τ (map Pos l)) ≠ nat.bodd (count_neg c) 
-    → clause.eval τ c = tt :=
-assume hc hcount, 
-  eval_tt_of_tt_ne_neg_of_map_var_eq hc (ne_of_apply_ne nat.bodd hcount)
+theorem eval_tt_of_map_var_eq_of_ne_parity {τ : assignment V} {l : list V} {c : clause V} : 
+  map var c = l → (clause.count_tt τ (map Pos l)).bodd ≠ (count_neg c).bodd → c.eval τ = tt :=
+λ hc hcount, eval_tt_of_map_var_eq_of_tt_ne_neg hc (ne_of_apply_ne nat.bodd hcount)
 
 -- Parity reasoning based on flips rather than negs
--- If a clause evaluates to false, then any clause that can be made by flipping a
--- variable in that clause will evaluate to true
 theorem eval_tt_of_ne_flips {τ : assignment V} {c₁ c₂ : clause V} :
-  map var c₁ = map var c₂ → 
-    c₁.count_tt τ ≠ count_flips c₁ c₂ → c₂.eval τ = tt :=
+  map var c₁ = map var c₂ → c₁.count_tt τ ≠ count_flips c₁ c₂ → c₂.eval τ = tt :=
 begin
   induction c₁ with l ls ih generalizing c₂,
   { simp },
@@ -657,38 +506,35 @@ begin
     { cases h : (τ m),
       { cases l;
         { unfold var at hm,
-          simp [count_tt_cons, count_flips_cons, 
-            literal.eval, literal.flip, ← hm, h] at hne,
+          simp [literal.eval, literal.flip, ← hm, h] at hne,
           exact eval_tt_cons_of_eval_tt _ (ih hms.symm hne) } },
       { simp only [eval_cons, literal.eval, hm, h, tt_bor] } },
     { cases h : (τ m),
       { simp only [eval_cons, literal.eval, hm, h, bnot, tt_bor] },
       { cases l;
         { unfold var at hm,
-          simp [count_tt_cons, count_flips_cons, 
-            literal.eval, literal.flip, ← hm, h] at hne,
+          simp [literal.eval, literal.flip, ← hm, h] at hne,
           exact eval_tt_cons_of_eval_tt _ (ih hms.symm hne) } } } }
 end
 
-/-! # vars -/
+end flips
 
--- Extract the set of variables in the clause
--- As all properties are set-like properties, use a finset
+/-! # vars -/
+section vars
+
+variables [decidable_eq V]
+
 protected def vars : clause V → finset V
 | []        := ∅
-| (l :: ls) := {l.var} ∪ (vars ls) -- Use insert instead?
+| (l :: ls) := {l.var} ∪ (vars ls) 
+--| (l :: ls) := insert l.var (vars ls) -- Use insert instead?
 
 @[simp] theorem vars_nil : clause.vars ([] : clause V) = ∅ := rfl
 
-@[simp] theorem vars_singleton (l : literal V) : clause.vars [l] = {l.var} :=
-by { unfold clause.vars, rw finset.union_empty }
+@[simp] theorem vars_singleton (l : literal V) : clause.vars [l] = {l.var} := rfl
 
-theorem mem_vars_cons_self (l : literal V) (c : clause V) :
-  l.var ∈ clause.vars (l :: c) :=
-begin
-  rw clause.vars,
-  exact finset.mem_union_left _ (finset.mem_singleton_self l.var)
-end
+theorem mem_vars_cons_self (l : literal V) (c : clause V) : l.var ∈ clause.vars (l :: c) :=
+finset.mem_union_left _ (finset.mem_singleton_self l.var)
 
 theorem mem_vars_cons_of_mem_vars {c : clause V} (l : literal V) {v : V} : 
   v ∈ c.vars → v ∈ clause.vars (l :: c) :=
@@ -698,7 +544,7 @@ theorem vars_append (c₁ c₂ : clause V) : (c₁ ++ c₂).vars = c₁.vars ∪
 begin
   induction c₁ with l ls ih,
   { simp only [finset.empty_union, vars_nil, nil_append] },
-  { simp only [cons_append, clause.vars, ih, finset.union_assoc] }
+  { simp only [cons_append, clause.vars, ih, finset.union_assoc], }
 end
 
 theorem vars_perm {c₁ c₂ : clause V} : c₁ ~ c₂ → c₁.vars = c₂.vars :=
@@ -706,9 +552,9 @@ begin
   intro hp,
   induction hp with x l₂ l₂' p IH  x y l₂  l₂ m₂ r₂ p₁ p₂ IH₁ IH₂,
   { refl },
-  { simp [clause.vars, IH] },
-  { simp [clause.vars, ← finset.union_assoc],
-    rw finset.union_comm {x.var} {y.var} },
+  { unfold clause.vars, rw IH },
+  { unfold clause.vars,
+    rw [← finset.union_assoc, ← finset.union_assoc, finset.union_comm {x.var} {y.var}] },
   { exact eq.trans IH₁ IH₂ }
 end
 
@@ -732,25 +578,25 @@ begin
     { use [l, mem_cons_self l ls, h] },
     { rcases finset.mem_union.mp hmem with h₁| h₂,
       { exact absurd (finset.mem_singleton.mp h₁).symm h },
-      { rcases ih h₂ with ⟨m, hm, hv⟩,
-        use [m, mem_cons_of_mem l hm, hv] } } }
+      { rcases ih h₂ with ⟨m, hm, hv⟩, use [m, mem_cons_of_mem l hm, hv] } } }
 end
 
-theorem vars_subset_of_vars_cons (l : literal V) (c : clause V) :
-  c.vars ⊆ clause.vars (l :: c) :=
+theorem vars_subset_of_vars_cons (l : literal V) (c : clause V) : c.vars ⊆ clause.vars (l :: c) :=
 finset.subset_union_right _ _
 
-theorem vars_subset_of_subset {c₁ c₂ : clause V} :
-  c₁ ⊆ c₂ → c₁.vars ⊆ c₂.vars :=
+theorem vars_subset_of_subset {c₁ c₂ : clause V} : c₁ ⊆ c₂ → c₁.vars ⊆ c₂.vars :=
 begin
   intros h v hv,
   rcases exists_mem_clause_of_mem_vars hv with ⟨l, hl, rfl⟩,
   exact mem_vars_of_mem (h hl)
 end
 
+section mem_vars_lemmas
+
+variables {v : V} {c : clause V}
+
 -- (map var c) and vars c are equivalent from a set perspective
-theorem mem_vars_iff_mem_map_vars {c : clause V} {v : V} :
-  v ∈ c.vars ↔ v ∈ map var c :=
+theorem mem_vars_iff_mem_map_vars : v ∈ c.vars ↔ v ∈ map var c :=
 begin
   split,
   { intro h,
@@ -760,91 +606,54 @@ begin
     exact hv ▸ mem_vars_of_mem hmem }
 end
 
-theorem not_mem_vars_iff_not_mem_map_vars {c : clause V} {v : V} :
-  v ∉ map var c ↔ v ∉ c.vars :=
+theorem not_mem_vars_iff_not_mem_map_vars : v ∉ map var c ↔ v ∉ c.vars :=
 by simp [mem_vars_iff_mem_map_vars]
 
-theorem mem_vars_iff_pos_or_neg_mem_clause {c : clause V} {v : V} :
-  v ∈ c.vars ↔ (Pos v) ∈ c ∨ (Neg v) ∈ c :=
+theorem mem_vars_iff_pos_or_neg_mem_clause : v ∈ c.vars ↔ (Pos v) ∈ c ∨ (Neg v) ∈ c :=
 begin
   split,
   { intro h,
     rcases exists_mem_clause_of_mem_vars h with ⟨l, hmem, hv⟩,
     cases l; { rw ← hv, simp [var, hmem] } },
-  { rintros (h | h);
-    { exact mem_vars_of_mem h } }
+  { rintros (h | h); { exact mem_vars_of_mem h } }
 end
 
-theorem vars_append_subset_left (c₁ c₂ : clause V) :
-  clause.vars c₁ ⊆ clause.vars (c₁ ++ c₂) :=
-begin
-  intros v hv,
-  rcases mem_vars_iff_pos_or_neg_mem_clause.mp hv with hv | hv;
-  { have := mem_vars_of_mem (mem_append_left _ hv),
-    assumption },
-end
+theorem vars_append_subset_left (c₁ c₂ : clause V) : c₁.vars ⊆ (c₁ ++ c₂).vars :=
+by { rw vars_append, exact finset.subset_union_left _ _ }
 
-theorem vars_append_subset_right (c₁ c₂ : clause V) :
-  clause.vars c₂ ⊆ clause.vars (c₁ ++ c₂) :=
-begin
-  intros v hv,
-  rcases mem_vars_iff_pos_or_neg_mem_clause.mp hv with hv | hv;
-  { have := mem_vars_of_mem (mem_append_right _ hv),
-    assumption },
-end
+theorem vars_append_subset_right (c₁ c₂ : clause V) : c₂.vars ⊆ (c₁ ++ c₂).vars :=
+by { rw vars_append, exact finset.subset_union_right _ _ }
 
-theorem mem_vars_append_left {v : V} {c₁ : clause V} (c₂ : clause V) :
-  v ∈ clause.vars c₁ → v ∈ clause.vars (c₁ ++ c₂) :=
+theorem mem_vars_append_left {c₁ : clause V} (c₂) : v ∈ c₁.vars → v ∈ (c₁ ++ c₂).vars :=
 assume h, vars_append_subset_left c₁ c₂ h
 
-theorem mem_vars_append_right {v : V} (c₁ : clause V) {c₂ : clause V} :
-  v ∈ clause.vars c₂ → v ∈ clause.vars (c₁ ++ c₂) :=
+theorem mem_vars_append_right (c₁) {c₂ : clause V} : v ∈ c₂.vars → v ∈ (c₁ ++ c₂).vars :=
 assume h, vars_append_subset_right c₁ c₂ h
 
-theorem mem_left_or_right_of_mem_vars_append {v : V} {c₁ c₂ : clause V} :
-  v ∈ clause.vars (c₁ ++ c₂) → (v ∈ clause.vars c₁) ∨ (v ∈ clause.vars c₂) :=
-begin
-  intro h,
-  rcases exists_mem_clause_of_mem_vars h with ⟨l, hl, rfl⟩,
-  rcases mem_append.mp hl with hl | hl;
-  { simp [mem_vars_of_mem hl] }
-end
+theorem mem_left_or_right_of_mem_vars_append {c₁ c₂ : clause V} :
+  v ∈ (c₁ ++ c₂).vars → (v ∈ c₁.vars) ∨ (v ∈ c₂.vars) :=
+by { rw vars_append, exact finset.mem_union.mp }
 
-theorem not_mem_vars_append_left {v : V} {c₁ c₂ : clause V} :
-  v ∉ clause.vars (c₁ ++ c₂) → v ∉ clause.vars c₁ :=
-begin
-  contrapose,
-  simp,
-  exact mem_vars_append_left c₂
-end
+theorem not_mem_vars_append_left {c₁ c₂ : clause V} : v ∉ (c₁ ++ c₂).vars → v ∉ c₁.vars :=
+assume h, mt (mem_vars_append_left c₂) h
 
-theorem not_mem_vars_append_right {v : V} {c₁ c₂ : clause V} :
-  v ∉ clause.vars (c₁ ++ c₂) → v ∉ clause.vars c₂ :=
-begin
-  contrapose,
-  simp,
-  exact mem_vars_append_right c₁
-end
+theorem not_mem_vars_append_right {c₁ c₂ : clause V} : v ∉ (c₁ ++ c₂).vars → v ∉ c₂.vars :=
+assume h, mt (mem_vars_append_right c₁) h
 
-theorem not_mem_vars_append_of_not_mem_of_not_mem {v : V} {c₁ c₂ : clause V} :
-  v ∉ clause.vars c₁ → v ∉ clause.vars c₂ → v ∉ clause.vars (c₁ ++ c₂) :=
+theorem not_mem_vars_append_of_not_mem_of_not_mem {c₁ c₂ : clause V} :
+  v ∉ c₁.vars → v ∉ c₂.vars → v ∉ (c₁ ++ c₂).vars :=
 begin
   intros h₁ h₂ hcon,
-  rcases mem_left_or_right_of_mem_vars_append hcon with hv | hv;
-  { contradiction }
+  rcases mem_left_or_right_of_mem_vars_append hcon; { contradiction }
 end
 
-end clause
+end mem_vars_lemmas
 
-/-! # eqod for clauses -/
+open assignment
 
-namespace assignment
+variables {τ₁ τ₂ : assignment V} {c : clause V}
 
-open literal
-open clause
-
-theorem eval_eq_clause_of_eqod {τ₁ τ₂ : assignment V} {c : clause V} :
-  (eqod τ₁ τ₂ c.vars) → c.eval τ₁ = c.eval τ₂ :=
+theorem eval_eq_of_eqod : (eqod τ₁ τ₂ c.vars) → c.eval τ₁ = c.eval τ₂ :=
 begin
   intro h,
   cases hev : (c.eval τ₂),
@@ -855,27 +664,23 @@ begin
   { rcases eval_tt_iff_exists_literal_eval_tt.mp hev with ⟨l, hl, htt⟩,
     apply eval_tt_iff_exists_literal_eval_tt.mpr,
     use [l, hl],
-    exact htt ▸ eval_eq_of_eqod_of_var_mem h (mem_vars_of_mem hl) }
+    exact htt ▸ eval_eq_of_eqod_of_var_mem h (mem_vars_of_mem hl) }  
 end
 
--- Can replace τ in count_tt if eqod
-theorem count_tt_eq_of_eqod {τ₁ τ₂ : assignment V} {c : clause V} :
-  (eqod τ₁ τ₂ c.vars) → clause.count_tt τ₁ c = clause.count_tt τ₂ c :=
+theorem count_tt_eq_of_eqod : (eqod τ₁ τ₂ c.vars) → c.count_tt τ₁ = c.count_tt τ₂ :=
 begin
   induction c with l ls ih,
   { simp only [count_tt_nil, eqod_nil, vars_nil, forall_true_left] },
   { intro h,
     rw clause.vars at h,
-    have ihred := ih (eqod_right_of_eqod_union h),
     cases l;
-    { have := eqod_left_of_eqod_union h,
-      rw literal.var at this,
-      simp [count_tt_cons, literal.eval, 
-        this l (finset.mem_singleton_self l), ihred] } }
+    { rw literal.var at h,
+      simp [literal.eval, eqod_union_left h l (finset.mem_singleton_self l), ih (eqod_union_right h)] } }
 end
 
-theorem count_tt_ite {τ₁ τ₂ : assignment V} (c : clause V) :
-  clause.count_tt (assignment.ite c.vars τ₁ τ₂) c = clause.count_tt τ₁ c :=
+theorem count_tt_ite (c : clause V) : c.count_tt (assignment.ite c.vars τ₁ τ₂) = c.count_tt τ₁ :=
 count_tt_eq_of_eqod (ite_eqod c.vars τ₁ τ₂)
 
-end assignment
+end vars
+
+end clause
