src/cnf/literal.lean
@@ -54,18 +54,8 @@ def var : literal V → V
 theorem var_surjective : surjective (var : literal V → V) :=
 assume v, exists.intro (Pos v) (by simp only [var])
 
-theorem ne_of_ne_var {l₁ l₂ : literal V} :
-  l₁.var ≠ l₂.var → l₁ ≠ l₂ :=
+theorem ne_of_ne_var {l₁ l₂ : literal V} : l₁.var ≠ l₂.var → l₁ ≠ l₂ :=
 assume h₁ h₂, h₁ (congr_arg var h₂)
-
--- Cases on l gives this immediately, so a kind of shorthand
-theorem pos_or_neg_of_var_eq_nat {l : literal V} {v : V} :
-  l.var = v → l = (Pos v) ∨ l = (Neg v) :=
-begin
-  cases l,
-  { simp only [var], exact or.intro_left false },
-  { simp only [var], exact or.intro_right false }
-end
 
 /-! # Evaluation -/
 
@@ -81,84 +71,59 @@ protected def eval (τ : assignment V) : literal V → bool
 /-! # Flip -/
 
 /- Flips the parity of the literal from positive to negative and vice versa -/
--- Protected because "flip" exists already as a way to interchange
--- the order of curried arguments
 protected def flip : literal V → literal V
 | (Pos v) := Neg v
 | (Neg v) := Pos v
 
-@[simp] theorem flip_ne [decidable_eq V] (l : literal V) : l.flip ≠ l :=
-by cases l; unfold literal.flip; exact dec_trivial
+@[simp] theorem flip_ne [decidable_eq V] : ∀ (l : literal V), l.flip ≠ l
+| (Pos v) := dec_trivial
+| (Neg v) := dec_trivial
 
-theorem flip_flip (l : literal V) : l.flip.flip = l :=
-by cases l; simp only [literal.flip]
+theorem flip_flip : ∀ (l : literal V), l.flip.flip = l
+| (Pos v) := rfl
+| (Neg v) := rfl
 
-theorem flip_var_eq (l : literal V) : l.flip.var = l.var :=
-by cases l; simp only [literal.flip, var]
+theorem flip_var_eq : ∀ (l : literal V), l.flip.var = l.var
+| (Pos v) := rfl
+| (Neg v) := rfl
 
-@[simp] theorem flip_injective : 
-  injective (literal.flip : literal V → literal V) :=
+@[simp] theorem flip_injective : injective (literal.flip : literal V → literal V) :=
 assume l₁ l₂ h, (flip_flip l₂) ▸ ((flip_flip l₁) ▸ (congr_arg literal.flip h))
 
 theorem flip_inj {l₁ l₂ : literal V} : l₁.flip = l₂.flip ↔ l₁ = l₂ :=
 flip_injective.eq_iff
 
-@[simp] theorem flip_surjective : 
-  surjective (literal.flip : literal V → literal V) :=
+@[simp] theorem flip_surjective : surjective (literal.flip : literal V → literal V) :=
 assume l, exists.intro l.flip (flip_flip l)
 
-@[simp] theorem flip_bijective : 
-  bijective (literal.flip : literal V → literal V) :=
+@[simp] theorem flip_bijective : bijective (literal.flip : literal V → literal V) :=
 ⟨flip_injective, flip_surjective⟩
 
 theorem exists_flip_eq (l₁ : literal V) : ∃ (l₂ : literal V), l₂.flip = l₁ :=
-begin
-  use l₁.flip,
-  rw flip_flip
-end
+⟨l₁.flip, flip_flip l₁⟩
 
--- Various lemmas on how var and flip interact
+section -- Various lemmas on how var and flip interact
 
-theorem var_eq_iff_eq_or_flip_eq {l₁ l₂ : literal V} : 
-  l₁.var = l₂.var ↔ l₁ = l₂ ∨ l₁.flip = l₂ :=
-begin
-  split,
-  { cases l₁; { cases l₂; simp [literal.flip, var] }},
-  { intro h, cases h,
-    { exact congr_arg var h },
-    { exact congr_arg var h ▸ (flip_var_eq l₁).symm } }
-end
+variables {l₁ l₂ : literal V}
 
-theorem flip_eq_iff_eq_flip {l₁ l₂ : literal V} : 
-  l₁.flip = l₂ ↔ l₁ = l₂.flip :=
+theorem var_eq_iff_eq_or_flip_eq : l₁.var = l₂.var ↔ l₁ = l₂ ∨ l₁.flip = l₂ :=
+by cases l₁; cases l₂; simp [literal.flip, var]
+
+theorem flip_eq_iff_eq_flip : l₁.flip = l₂ ↔ l₁ = l₂.flip :=
 ⟨λ h, congr_arg literal.flip h ▸ (flip_flip l₁).symm, 
  λ h, (congr_arg literal.flip h).symm ▸ flip_flip l₂⟩
 
-theorem flip_ne_iff_ne_flip {l₁ l₂ : literal V} :
-  l₁.flip ≠ l₂ ↔ l₁ ≠ l₂.flip :=
-begin
-  split;
-  { contrapose,
-    simp [flip_eq_iff_eq_flip] },
-end
+theorem flip_ne_iff_ne_flip : l₁.flip ≠ l₂ ↔ l₁ ≠ l₂.flip :=
+⟨λ h₁ h₂, absurd (flip_eq_iff_eq_flip.mpr h₂) h₁, 
+ λ h₁ h₂, absurd (flip_eq_iff_eq_flip.mp h₂) h₁⟩
 
-theorem flip_eq_of_ne_of_var_eq {l₁ l₂ : literal V} :
-  l₁ ≠ l₂ → l₁.var = l₂.var → l₁.flip = l₂ :=
-begin
-  intros h₁ h₂,
-  cases var_eq_iff_eq_or_flip_eq.mp h₂,
-  { contradiction },
-  { exact h }
-end
+theorem flip_eq_of_ne_of_var_eq : l₁ ≠ l₂ → l₁.var = l₂.var → l₁.flip = l₂ :=
+λ h₁ h₂, or.elim (var_eq_iff_eq_or_flip_eq.mp h₂) (λ h, absurd h h₁) id
 
-theorem eq_of_flip_ne_of_var_eq {l₁ l₂ : literal V} :
-  l₁.flip ≠ l₂ → l₁.var = l₂.var → l₁ = l₂ :=
-begin
-  intros h₁ h₂,
-  cases var_eq_iff_eq_or_flip_eq.mp h₂,
-  { exact h },
-  { contradiction }
-end
+theorem eq_of_flip_ne_of_var_eq : l₁.flip ≠ l₂ → l₁.var = l₂.var → l₁ = l₂ :=
+λ h₁ h₂, or.elim (var_eq_iff_eq_or_flip_eq.mp h₂) id (λ h, absurd h h₁)
+
+end /- end section -/
 
 /-! # Flip evaluation -/
 
@@ -198,33 +163,21 @@ protected def is_false (τ : assignment V) (l : literal V) : Prop :=
 literal.eval τ l = ff
 
 -- is_pos, etc. are decidable
-instance : decidable_pred (literal.is_pos : literal V → Prop) :=
-begin
-  intro l, cases l,
-  { unfold literal.is_pos, exact decidable.true },
-  { unfold literal.is_pos, exact decidable.false }
-end
+instance : decidable_pred (literal.is_pos : literal V → Prop)
+| (Pos v) := decidable.true
+| (Neg v) := decidable.false
 
-instance : decidable_pred (literal.is_neg : literal V → Prop) :=
-begin
-  intro l, cases l,
-  { unfold literal.is_neg, exact decidable.false },
-  { unfold literal.is_neg, exact decidable.true }
-end
+instance : decidable_pred (literal.is_neg : literal V → Prop)
+| (Pos v) := decidable.false
+| (Neg v) := decidable.true
 
 instance (τ : assignment V) : decidable_pred (literal.is_true τ) :=
-begin
-  intro l,
-  cases h : literal.eval τ l;
+λ l, by cases h : literal.eval τ l;
   { unfold literal.is_true, rw h, exact eq.decidable _ _ }
-end
 
 instance (τ : assignment V) : decidable_pred (literal.is_false τ) :=
-begin
-  intro l,
-  cases h : literal.eval τ l;
+λ l, by cases h : literal.eval τ l;
   { unfold literal.is_false, rw h, exact eq.decidable _ _ }
-end
 
 -- A literal can never be both positive and negative
 theorem is_pos_ne_is_neg (l : literal V) :
